updataing main branch with up to date version
more info in README

paper.pdf added

theories/env.v
@@ -1,107 +1,114 @@
-(* Imported libraries *) 
 From mathcomp Require Import all_ssreflect.
 From Coq Require Import FunctionalExtensionality.
-Require Import free_names types semantics syntax fintype core linearity_predicate.
+Require Import free_names types synsem.
 
+Section TotalMap.
+  Variables (K : eqType) (A : Type).
+
+  Definition total_map := K -> A.
+  
+  Definition t_update (m : total_map) (x : K) (v : A) : total_map :=
+    fun y => if y == x then v else m y.
+  
+  Lemma t_update_others (m : total_map) x y v :
+    y <> x -> t_update m x v y = m y.
+  Proof. move=> Hyx; rewrite /t_update. case eqP => //=. Qed.
+
+  Theorem t_update_swap : forall  (m : total_map ) v1 v2 x1 x2,
+      x2 <> x1 ->
+      (t_update (t_update m x2 v2) x1 v1) =
+         (t_update (t_update m x1 v1) x2 v2).
+      Proof.
+    intros  m v1 v2 x1 x2 H.
+    apply functional_extensionality. intros x3.
+    rewrite /t_update => //=.
+    case eqP => //=.
+    intro c.
+    case eqP => //=.
+    intro d.
+    rewrite <- d in H.
+    contradiction.
+  Qed.
+
+(* Other lemmas, SF-style, unused *)
+  Lemma t_update_same (m : total_map) x : t_update m x (m x) = m.
+  Proof. 
+    by apply/functional_extensionality  => y; rewrite /t_update; case: eqP => // ->. 
+  Qed.
+
+  Lemma t_update_eq (m : total_map) x v : t_update m x v x = v.
+  Proof. by rewrite /t_update eqxx. Qed.
+
+   Lemma t_update_shadow : forall (m : total_map ) x v1 v2,
+   (t_update (t_update m x v1) x v2) =
+  (t_update m x v2).
+  Proof.
+    intros  m x v1 v2. apply functional_extensionality. intros x'.  unfold t_update.    case: eqP => // ->. 
+  Qed.
+ 
+End TotalMap.
+
+Notation "x '!!->' v ';' m" :=
+  (t_update _ _ m x v)
+    (at level 100, v at next level, right associativity).
+  
 
 Definition env (n:nat) := ch n -> sType.
 
-Definition update {n : nat} (e : env n) (x : ch n) (T : sType) : 
-  env n := fun y => if (x==y) then T else e y.
-
-Notation "x '!->' v ';' m" := (update m x v)
-                              (at level 100, v at next level, right associativity).
-
-Lemma update_others {n : nat}: forall c x T (Delta : env n),
-    c <> x -> update Delta x T c = Delta c. 
-Proof. 
-  move => c x T Delta H.
-  rewrite/update. 
-  by case: ifP => // => /eqP => Hyp; subst.
-Qed. 
-
-Lemma update_swap {n : nat}: forall x T1 y T2 (Delta : env n),
-    x<>y -> update (update Delta x T1) y T2 = 
-              update (update Delta y T2) x T1. 
-Proof.
-  move => x T1 y T2 Delta H.
-  apply/functional_extensionality => x0.
-  rewrite/update.
-  case: ifP.
-  - move/eqP => H'; subst. 
-    case: ifP => //.
-    move/eqP => //.
-  - move/eqP => H'. 
-    case: ifP => //.
-Qed. 
-
-
-Definition shift_env {n : nat} (T : sType) (e : env n) : env n.+1 :=
-  fun x => match x with
-           | var_ch None => T
-           | var_ch (Some i) => e (var_ch i)
-           end.
-Check scons.
+Definition shift_env {n : nat} (T : sType) (e : env n) : env n.+1 := scons  T e.
+  
 Notation "T ::: Delta" := (shift_env T Delta) (at level 40).
 
-
-Lemma update_var_zero {n : nat}: forall T1 T2 Delta,
-    (update (shift_env T1 Delta) (n.+2__ch var_zero) T2) 
-    = (shift_env T2 Delta). 
+Lemma update_zero {n : nat}: forall T1 T2 Delta,
+    (t_update _ _ (shift_env T1 Delta) zero T2) = (@shift_env n T2 Delta). 
 Proof.
   move => T1 T2 Delta. 
   apply/functional_extensionality => x0.
   destruct x0 => //.
-  destruct f => //.
 Qed. 
 
-Lemma update_var_one {n : nat}: forall T1 T2 T Delta,
-    (update (shift_env T1 (shift_env T2 Delta)) (n.+2__ch var_one) T) 
-    = (shift_env T1 (shift_env T Delta)). 
+Lemma update_one {n : nat}: forall T1 T2 T Delta,
+    (t_update _ _ (shift_env T1 (shift_env T2 Delta)) one T) 
+    = (shift_env T1 ( @shift_env n T Delta)). 
 Proof.
   move => T1 T2 T Delta. 
   apply/functional_extensionality => x0.
   destruct x0 => //.
-  destruct f => //.
-  destruct f => //.
+  destruct c => //.
 Qed. 
 
-Lemma update_var_two {n : nat}: forall T1 T2 T3 T Delta,
-    (update (shift_env T1 (shift_env T2 (shift_env T3 Delta)))
-       (n.+3__ch var_two) T) 
-    = (shift_env T1 (shift_env T2 (shift_env T Delta))). 
+Lemma update_two {n : nat}: forall T1 T2 T3 T Delta,
+    (t_update _ _
+       (shift_env T1 (shift_env T2 (shift_env T3 Delta))) two T)
+    = (shift_env T1 (shift_env T2 (@shift_env n T Delta))). 
 Proof.
   move => T1 T2 T3 T Delta. 
   apply/functional_extensionality => x0.
   destruct x0 => //.
-  destruct f => //.
-  destruct f => //.
-  destruct f => //.
+  destruct c => //.
+  destruct c => //.
 Qed. 
 
-Lemma shift_env_update {n : nat}: forall i T1 T2 (Delta : env n),
-    shift_env T1 (update Delta (var_ch i) T2) = 
-      update (shift_env T1 Delta) (var_ch (shift i)) T2. 
+Lemma shift_env_update {n : nat}: forall x T1 T2 (Delta : env n),
+    shift_env T1 (t_update _ _ Delta x T2) =
+      t_update _ _ (shift_env T1 Delta) (shift x) T2. 
 Proof. 
-  move => i T1 T2 Delta.
+  move => x T1 T2 Delta.
   apply/functional_extensionality => x0.
-  rewrite/shift_env/update => /=.
+  rewrite/shift_env/t_update => /=.
   case: ifP. 
-  - move/eqP => <- /=.
+  - move/eqP => -> /=.
     case: ifP => //.
     move/eqP => //.
-  - destruct x0 => //.
-    destruct f => //.
-    move/eqP.
+  - destruct x0 => //=.
+    move/eqP => H.
     case: ifP => //.
-    move/eqP.
-    case => ->.
-    case => //.
-Qed. 
-
+    move/eqP => H'; subst => //.
+Qed.
+  
 (* Relation between typing environments *) 
-Definition ltc {n m} (Delta: env n) (Gamma: env m) (sigma : fin n -> ch m) P := 
-  forall i, free_in (var_ch i) P -> Delta (var_ch i) = Gamma (sigma i).
+Definition ltc {n m} (Delta: env n) (Gamma: env m) (sigma : ch n -> ch m) P := 
+  forall x, free_in x P -> Delta  x = Gamma (sigma x).
 
 Lemma ltc_WaitP {n m}: forall {Delta: env n} {Gamma: env m} sigma x P, 
     ltc Delta Gamma sigma (WaitP x P) -> ltc Delta Gamma sigma P.
@@ -123,23 +130,21 @@ Lemma ltc_ResP {n m}: forall T1 T2 {Delta: env n} {Gamma: env m} sigma P,
     ltc Delta Gamma sigma (ResP P) -> 
     ltc (shift_env T1 (shift_env T2 Delta)) 
       (shift_env T1 (shift_env T2 Gamma)) 
-      (up_ch_ch (up_ch_ch sigma))
+      (up_ch (up_ch sigma))
       P.
 Proof.
   move => T1 T2 Delta Gamma sigma P. 
-  rewrite/ltc/shift_env => H i Hyp.
-  destruct i => //=. 
-  destruct f => //.
+  rewrite/ltc/shift_env => H x Hyp.
+  destruct x => //=. 
+  destruct c => //=.
   rewrite H => //=. 
-  rewrite/up_ch_ch/funcomp => /=. 
-  destruct (sigma f) => //.
 Qed.
 
 Lemma ltc_ParPL {n m}: forall {Delta: env n} {Gamma: env m} sigma P Q, 
     ltc Delta Gamma sigma (ParP P Q) -> ltc Delta Gamma sigma P.
 Proof.
   move => Delta Gamma sigma P Q H. 
-  rewrite/ltc => i H'.
+  rewrite/ltc => x H'.
   by apply/H => /=; left.
 Qed. 
 
@@ -147,21 +152,17 @@ Lemma ltc_ParPR {n m}: forall {Delta: env n} {Gamma: env m} sigma P Q,
     ltc Delta Gamma sigma (ParP P Q) -> ltc Delta Gamma sigma Q.
 Proof.
   move => Delta Gamma sigma P Q H. 
-  rewrite/ltc => i H'.
+  rewrite/ltc => x H'.
   by apply/H => /=; right.
 Qed. 
 
 Lemma ltc_InSP {n m}: forall T {Delta: env n} {Gamma: env m} sigma x P, 
     ltc Delta Gamma sigma (InSP x P) -> 
-    ltc (shift_env T Delta) (shift_env T Gamma) (up_ch_ch sigma) P.
+    ltc (shift_env T Delta) (shift_env T Gamma) (up_ch sigma) P.
 Proof.
-  move => T Delta Gamma sigma x P.
-  rewrite/ltc/shift_env => H i Hyp.  
-  destruct i => //=. 
-  rewrite H => /=.
-  rewrite/funcomp. 
-  by destruct (sigma f).
-  by right. 
+  move => T Delta Gamma sigma x P H y Hyp.  
+  destruct y => //.
+  by apply/H; right.
 Qed. 
 
 Lemma ltc_DelP {n m}: forall {Delta: env n} {Gamma: env m} sigma x y P, 
@@ -174,7 +175,7 @@ Qed.
 
 Lemma ltc_scons {n : nat} : forall x T Delta P,
     Delta x = T -> 
-    ltc (shift_env T Delta)  Delta (scons x n __ch) P.
+    @ltc n.+1 n (shift_env T Delta) Delta (scons x id_ren) P.
 Proof.
   move => x T Delta P H.
   rewrite/shift_env/ltc => k'.
@@ -184,13 +185,13 @@ Qed.
 Definition swap_env {n : nat} (Delta : env n) j k := 
   fun i => if i == j then Delta k else if i == k then Delta j else Delta i.
 
-Lemma ltc_swap {n : nat} : forall j k Delta Gamma (P : proc n), 
-    Gamma = (swap_env Delta (var_ch j) (var_ch k)) -> 
-    ltc Delta Gamma (swap_ch j k) P.
+Lemma ltc_swap {n : nat} : forall x y Delta Gamma (P : proc n), 
+    Gamma = (swap_env Delta x y) -> ltc Delta Gamma (swap_ch x y) P.
 Proof. 
-  rewrite/swap_env/swap_ch => j k Delta Gamma P H1 i H2; subst.
+  move => x y Delta Gamma P H1 i H2; subst.
+  rewrite/swap_env/swap_ch.
   case: ifP.
-  - move/eqP; case.
+  - move/eqP.
     case: ifP.
     by move/eqP => -> ->.
     move/eqP => H1.
@@ -205,31 +206,26 @@ Proof.
     case: ifP => //.
     move/eqP => H3 H4.
     case: ifP => //.
-    move/eqP; case => //.
+    move/eqP => H; subst => //.
 Qed. 
 
 (* Injectivity and update *) 
-Lemma ltc_update {k k'}: forall n T {Delta: env k} {Gamma: env k'} P sigma,
-    free_in (var_ch n) P -> 
+Lemma ltc_update {k k'}: forall x T {Delta: env k} {Gamma: env k'} P sigma,
+    free_in x P -> 
     injectiveS P sigma -> 
     ltc Delta Gamma sigma P -> 
-    ltc (update Delta (var_ch n) T) (update Gamma (sigma n) T) sigma P.
+    ltc (t_update _ _ Delta x T)
+      (t_update _ _ Gamma (sigma x) T) sigma P.
 Proof. 
-  move => n T Delta Gamma P sigma Hfree H1.
-  rewrite/ltc => H2 i. 
-  rewrite/update. 
+  move => x T Delta Gamma P sigma Hfree H1 H2 y H. 
+  rewrite/t_update. 
   case: ifP => /eqP.
-  + case => Hyp; subst. 
+  + move => Hyp; subst. 
     case: ifP => /eqP => //.
-  + move => Hyp1 Hyp2.
-    have fact : n <> i. 
-    move:Hyp1.
-    by apply/contra_not => ->.
+  + move => Hdiff.
     case : ifP.
-    move/eqP => /H1. 
-    move => H.
-    apply fact in H => //.
-    move => _.
-    rewrite H2 => //.
-Qed.
-
+    * move/eqP => /H1 => Hyp.
+      move:  (Hyp H Hfree) => Hyp' => //.
+    * move/eqP => Hdiff'.
+      rewrite H2 => //.
+Qed. 
