theories/linearity_predicate.v
@@ -1,278 +1,241 @@
 (* Imported libraries *) 
 From mathcomp Require Import all_ssreflect.
-Require Import core fintype free_names syntax semantics. 
+Require Import free_names synsem. 
 
 (* Linear Predicate *)
 Inductive lin {n : nat} : ch n -> proc n -> Prop :=
     LWaitP : forall (x : ch n) (P : proc n),
-             ~ free_in x P -> lin x (x ? ․ P)
+             ~(free_in x P) -> lin x (x ? ․ P)
   | LWaitPcongr : forall (x y : ch n) (P : proc n),
                   lin y P -> x <> y -> lin y (x ? ․ P)
   | LCloseP : forall (x : ch n) (P : proc n),
-              ~ free_in x P -> lin x (x ! ․ P)
+              ~(free_in x P) -> lin x (x ! ․ P)
   | LClosePcongr : forall (x y : ch n) (P : proc n),
                    lin y P -> x <> y -> lin y (x ! ․ P)
   | LResP : forall (x : ch n) (P : proc n.+2),
-  lin (subst_ch (fun i => var_ch (shift (shift i))) x) P ->
+  lin ((shift \o shift ) x) P ->
             lin x ((ν) P)
   | LParPL : forall (x : ch n) (P1 P2 : proc n),
              lin x P1 ->
-             ~ free_in x P2 -> lin x (P1 ∥ P2)
+             ~(free_in x P2) -> lin x (P1 ∥ P2)
   | LParPR : forall (x : ch n) (P1 P2 : proc n),
-             ~ free_in x P1 ->
+             ~(free_in x P1) ->
              lin x P2 -> lin x (P1 ∥ P2)
   | LInSP : forall (x y : ch n) (P : proc n.+1),
-            lin (subst_ch (fun i => var_ch (shift i)) y) P ->
+            lin (shift  y) P ->
              lin y (x ? (_)․P)
   | LDelP : forall (x y z : ch n) (P : proc n),
             z <> y -> lin z P -> lin z (x ! y ․ P)
   | LDelPObj : forall (x y : ch n) (P : proc n),
                x <> y ->
-               ~ free_in y P -> lin y (x ! y ․ P).
+               ~(free_in y P) -> lin y (x ! y ․ P).
 
 Lemma lin_subst {n : nat} {m : nat} : 
-  forall (i : fin n) y (P : proc n) (sigma : fin n -> ch m), 
-    lin (var_ch i) P -> 
-    injectiveNS i P sigma -> 
-    y = sigma i -> (* this just makes it easier applyin IH *)
+  forall (x : ch n) y (P : proc n) (sigma : ren n m), 
+    lin x P -> 
+    injectiveNS x P sigma -> 
+    y = sigma x -> (* this just makes it easier applyin IH *)
     lin y (subst_proc sigma P).
 Proof. 
-  move => i [j] P; elim: P m i j => /=.
+  move => x y P; elim: P m x y => /=.
   - by intros; inversion H.  
   (* WaitP *)
-  - move => n0 [j0] P IH m i j sigma => /= H1 => H2 H3.
+  - move => n0 c P IH m x y sigma => /= H1 => H2 H3.
     inversion H1; subst.
-    * rewrite H3 => {H3 j}. 
-      apply/LWaitP.
+    * apply/LWaitP.
       move:H4.
       apply/contra_not. 
-      move/(free_in_subst _ sigma); apply. 
-      by rewrite/injectiveNS => j' Hyp; apply/H2 => /=; right.
+      move/(free_in_subst_inv _ sigma); apply.
+      by move => j' Hyp; apply/H2 => /=; right.
     * apply/LWaitPcongr.
-      apply/(IH _ i j) => //.
-      by rewrite/injectiveNS => j' Hyp; apply/H2 => /=; right.
+      apply/(IH _ x) => //.
+      by move => y' Hyp; apply/H2 => /=; right.
       move: H6. 
-      apply/contra_not => Hyp.
-      f_equal.
+      apply/contra_not => Hyp. 
       apply/Logic.eq_sym. 
-      apply/H2 => //=. 
-      by left.  
-      by rewrite -H3.
+      apply/H2; firstorder. 
   (* CloseP *)
-  - move => n0 [j0] P IH m i j sigma => /= H1 => H2 H3.
+  - move => n0 c P IH m x y sigma => /= H1 => H2 H3.
     inversion H1; subst.
-    * rewrite H3 => {H3 j}. 
-      apply/LCloseP.
+    * apply/LCloseP.
       move:H4.
       apply/contra_not. 
-      move/(free_in_subst _ sigma); apply. 
-      by rewrite/injectiveNS => j' Hyp; apply/H2 => /=; right.
+      move/(free_in_subst_inv _ sigma); apply.
+      by move => j' Hyp; apply/H2 => /=; right.
     * apply/LClosePcongr.
-      apply/(IH _ i j) => //.
-      by rewrite/injectiveNS => j' Hyp; apply/H2 => /=; right.
+      apply/(IH _ x) => //.
+      by move => y' Hyp; apply/H2 => /=; right.
       move: H6. 
-      apply/contra_not => Hyp.
-      f_equal.
+      apply/contra_not => Hyp. 
       apply/Logic.eq_sym. 
-      apply/H2 => //=. 
-      by left.  
-      by rewrite -H3.
+      apply/H2; firstorder. 
   (* ResP *)
-  - move => n0 P IH m i j sigma H1 H2 H3.
+  - move => n0 P IH m x y sigma H1 H2 H3.
     inversion H1; subst.
-    apply/LResP => /=. 
-    apply/(IH _ (shift (shift i))) => //.
-    by apply/injectiveNS_up_ch_ch_ResP.
-    asimpl. 
-    by rewrite/funcomp -H3. 
+    apply/LResP.
+    apply/(IH _ (shift (shift x))) => //.
+    by apply/injectiveNS_ResP.
   (* ParP *)
-  - move => n0 P IH1 Q IH2 m i j sigma H1 H2 H3.
+  - move => n0 P IH1 Q IH2 m x y sigma H1 H2 H3.
     inversion H1; subst. 
     * apply/LParPL.
-      apply/(IH1 _ i) => //. 
-      by apply/(injectiveNS_up_ch_ch_ParPL _ _ Q).
+      apply/(IH1 _ x) => //. 
+      by apply/(injectiveNS_ParPL _ _ Q).
       move:H6.
       apply/contra_not => Hyp.
-      apply/(free_in_subst _ sigma).
-      move:Hyp.
-      by rewrite H3.
-      by apply/(injectiveNS_up_ch_ch_ParPR _ P).
+      apply/(free_in_subst_inv _ sigma) => //.
+      by apply/(injectiveNS_ParPR _ P).
     * apply/LParPR.
       move:H5.
       apply/contra_not => Hyp.
-      apply/(free_in_subst _ sigma).
-      move:Hyp.
-      by rewrite H3.
-      by apply/(injectiveNS_up_ch_ch_ParPL _ _ Q).
-      apply/(IH2 _ i) => //. 
-      by apply/(injectiveNS_up_ch_ch_ParPR _ P).
+      apply/(free_in_subst_inv _ sigma) => //.
+      by apply/(injectiveNS_ParPL _ _ Q).
+      apply/(IH2 _ x) => //. 
+      by apply/(injectiveNS_ParPR _ P).
   (* InSP *) 
-  - move => n0 c P IH m i j sigma H1 H2 H3. 
+  - move => n0 c P IH m x y sigma H1 H2 H3. 
     inversion H1; subst. 
     apply/LInSP.
-    apply/(IH _ (shift i)) => //.
-    by apply/(injectiveNS_up_ch_ch_InSP _ c). 
-    asimpl; rewrite/funcomp. 
-    by rewrite -H3.
+    apply/(IH _ (shift x)) => //.
+    by apply/(injectiveNS_InSP _ c). 
   (* DelP *) 
-  - move => n0 [c] [c0] P IH m i j sigma H1 H2 H3. 
-    inversion H1; subst => /=. 
+  - move => n0 c c0 P IH m x y sigma H1 H2 H3. 
+    inversion H1; subst.
     * apply/LDelP => /=.
-      rewrite H3. 
       move:H5.
       apply/contra_not => Hyp.
-      f_equal.
       apply/H2 => //. 
       by right; left. 
-      apply/(IH _ i) => //.
-      by apply/(injectiveNS_up_ch_ch_DelSP _ (var_ch c) (var_ch c0)).
-    * rewrite H3. 
-      apply/LDelPObj.
+      apply/(IH _ x) => //.
+      by apply/(injectiveNS_DelSP _ ( c) ( c0)).
+    * apply/LDelPObj.
       move:H5.
       apply/contra_not => Hyp.
-      f_equal.
       apply/Logic.eq_sym. 
       by apply/H2 => //=; left.
       move:H7.
       apply/contra_not.
-      move/free_in_subst. 
+      move/free_in_subst_inv. 
       apply.
-      by apply/(injectiveNS_up_ch_ch_DelSP _ (var_ch c) (var_ch c0)).
+      by apply/(injectiveNS_DelSP _ ( c) ( c0)).
 Qed.
 
 
-Lemma lin_key_subst {n : nat} : forall (j : fin n.+2) (P : proc n.+3), 
-    lin (var_ch var_zero) P -> 
-    ~( free_in (var_ch (shift j)) P) -> 
-    lin (var_ch j) (subst_proc (scons (var_ch j) ids) P).
-Proof. 
-  intros. 
-  apply/(lin_subst _ _ _ _ H).
-  rewrite/injectiveNS => j0 /=.
-  intros. 
-  case: (fin_eq_dec (shift j) j0). 
-  intros; subst => //. 
-  move: H2.
-  rewrite/scons => /=.
-  destruct j0 => //.
-  case => ->.
-  by case. 
-  by asimpl.
+Lemma lin_key_subst {n : nat} : forall (y : ch n.+2) (P : proc n.+3), 
+    lin zero P -> 
+    ~( free_in (shift y) P) -> 
+    lin y (subst_proc (scons y id_ren) P).
+Proof.
+  move => y P H1 H2. 
+  apply/(lin_subst _ _ _ _ H1) => //. 
+  move => y0 /=. 
+  case: (ch_eq_dec (shift y) y0). 
+  move => H3 H4 H5; subst.
+  firstorder. 
+  move => H3 H4 H5; subst.
+  destruct y0 => //. 
+  move : H5 => /=.
+  rewrite/id_ren/shift => H; subst. 
+  firstorder. 
 Qed. 
 
+
 Lemma lin_subst_inv {n : nat} {m : nat} : 
-  forall (i : fin n) y (P : proc n) (sigma : fin n -> ch m), 
+  forall (x : ch n) y (P : proc n) (sigma : ren n m), 
     lin y (subst_proc sigma P) ->
-    injectiveNS i P sigma -> 
-    y = sigma i -> (* this just makes it easier applyin IH *)
-    lin (var_ch i) P.
+    injectiveNS x P sigma -> 
+    y = sigma x -> (* this just makes it easier applyin IH *)
+    lin x P.
 Proof. 
-  move => i [j] P sigma; elim: P m i j sigma => /=.
+  move => x y P sigma; elim: P m x y sigma => /=.
   - intros; inversion H.
   (* WaitP *)
-  - move => n0 [j0] P IH m i j sigma /= H1 HInj H2.
+  - move => n0 c P IH m x y sigma H1 HInj H2.
     inversion H1; subst.
-    * have fact: i = j0.
-      apply/HInj.
-      by left.
-      by rewrite -H2.
+    * have Hyp: x = c by apply/HInj => //; left.
       subst. 
       apply/LWaitP.
       move:H3.
       apply/contra_not.
-      move/(free_in_subst_inv _ sigma).
-      by rewrite H.
-    * apply/LWaitPcongr => //.
-      apply/(IH _ i j sigma) => //.
-      rewrite/injectiveNS => j1 Hyp1 Hyp2.
+      move/(free_in_subst _ sigma) => //.
+    * apply/LWaitPcongr.
+      apply/(IH _ x (sigma x) sigma) => //.
+      move => j Hyp1 Hyp2.
       apply/HInj => //.
       by right. 
       move:H5.
-      apply/contra_not.
-      case => -> //.
+      by apply/contra_not => ->.
   (* CLoseP *)
-  - move => n0 [j0] P IH m i j sigma /= H1 HInj H2.
+  - move => n0 c P IH m x y sigma H1 HInj H2.
     inversion H1; subst.
-    * have fact: i = j0.
-      apply/HInj.
-      by left.
-      by rewrite -H2.
+    * have Hyp: x = c by apply/HInj => //; left.
       subst. 
       apply/LCloseP.
       move:H3.
       apply/contra_not.
-      move/(free_in_subst_inv _ sigma).
-      by rewrite H.
-    * apply/LClosePcongr => //.
-      apply/(IH _ i j sigma) => //.
-      rewrite/injectiveNS => j1 Hyp1 Hyp2.
+      move/(free_in_subst) => //.
+    * apply/LClosePcongr.
+      apply/(IH _ x (sigma x) sigma) => //.
+      move => j Hyp1 Hyp2.
       apply/HInj => //.
       by right. 
       move:H5.
-      apply/contra_not.
-      case => -> //.
+      by apply/contra_not => ->.
   (* ResP *)
-  - move => n0 P IH m i j sigma /= H1 HInj H2.
+  - move => n0 P IH m x y sigma H1 HInj H2.
     inversion H1; subst. 
     apply/LResP. 
-    apply/(IH _ (shift (shift i)) (shift (shift j)) 
-             (up_ch_ch (up_ch_ch sigma))) => //=.
-    by apply/injectiveNS_up_ch_ch_ResP.
-    by asimpl; rewrite/funcomp -H2.
+    apply/(IH _ (shift (shift x)) (shift (shift (sigma x))) 
+             (up_ch (up_ch sigma))) => //=.
+    by apply/injectiveNS_ResP.
   (* ParP *)
-  - move => n0 P IH1 Q IH2 m i j sigma /= H1 HInj H2.
+  - move => n0 P IH1 Q IH2 m x y sigma H1 HInj H2.
     inversion H1; subst. 
     * apply/LParPL.
-      apply/(IH1 _ i j sigma) => //. 
-      by apply/(injectiveNS_up_ch_ch_ParPL _ _ Q).
+      apply/(IH1 _ x (sigma x)) => //. 
+      apply/H4.
+      apply/(injectiveNS_ParPL _ _ Q) => //.
       move:H5.
       apply/contra_not.
-      move/(free_in_subst_inv _ sigma) => /=.
-      by rewrite H2.
+      move/(free_in_subst _ sigma) => //.
     * apply/LParPR.
       move:H4.
       apply/contra_not.
-      move/(free_in_subst_inv _ sigma) => /=.
-      by rewrite H2.
-      apply/(IH2 _ i j sigma) => //. 
-      by apply/(injectiveNS_up_ch_ch_ParPR _ P).
+      move/(free_in_subst _ sigma) => //.
+      apply/(IH2 _ x (sigma x)) => //. 
+      apply/H5.
+      apply/(injectiveNS_ParPR _ P) => //.
   (* InSP *)
-  - move => n0 [k] P IH m i j sigma /= H1 HInj H2. 
+  - move => n0 c P IH m x y sigma H1 HInj H2. 
     inversion H1; subst. 
     apply/LInSP => /=.
-    apply/(IH _ _ (shift j) (up_ch_ch sigma)) => //=.
-    by apply/(injectiveNS_up_ch_ch_InSP _ (var_ch k)).
-    rewrite/funcomp/shift => /=.
-    by rewrite -H2.
+    apply/(IH _ _ (shift (sigma x)) (up_ch sigma)) => //.
+    apply/(injectiveNS_InSP _ c) => //.
   (* DelP *)
-  - move => n0 [k] [k0] P IH m i j sigma /= H1 HInj H2. 
+  - move => n0 c c0 P IH m x y sigma H1 HInj H2. 
     inversion H1; subst. 
     + apply/LDelP.
       move:H4. 
-      apply/contra_not. 
-      by case => <-.
-      apply/(IH _ _ j sigma) => //.
-      by apply/(injectiveNS_up_ch_ch_DelSP _ (var_ch k) (var_ch k0)).
+      by apply/contra_not => ->. 
+      apply/(IH _ _ (sigma x) sigma) => //.
+      by apply/(injectiveNS_DelSP _ c c0).
     + (* need to prove that i = k0 *)
-      have fact : i = k0.
-      apply/HInj.
-      by right;left.
-      by rewrite -H0 H2.
+      have fact : x = c0.
+      apply/HInj => //.
+      by right; left.
       subst. 
       apply/LDelPObj.
       move:H4.
-      apply/contra_not.
-      by case => ->.
+      by apply/contra_not => ->.
       move:H6.
-      apply/contra_not => /(free_in_subst_inv _ sigma). 
-      by rewrite H0.
+      by apply/contra_not => /(free_in_subst _ sigma). 
 Qed. 
 
    
 Lemma lin_congruence {n : nat} : forall {x : ch n} P Q,
     struct_eq P Q -> lin x P <-> lin x Q.
 Proof.
-  move => [i] P Q H; elim: H i => //.
+  move => x P Q H; elim: H x => //.
   - move => n0 P0 Q0.
     split.
     * move => H. 
@@ -328,19 +291,15 @@ Proof.
         apply/LParPL =>//.
         move : H4. 
         apply/contra_not.
-        asimpl.
-        move/free_in_subst. 
+        move/(free_in_subst_inv _ (fun x => shift (shift x))).
         apply.
-        rewrite/injectiveNS => x0 H.
-        by case. 
+        apply/injectiveNS_shift_shift.
       + apply/LResP.
         apply LParPR. 
         move : H3 => //=. 
-        asimpl. 
-        apply/(lin_subst) => //.
+        apply/lin_subst => //.
         apply/H4.
-        rewrite/injectiveNS => n0 H. 
-        by case. 
+        apply/injectiveNS_shift_shift.
     }
     { move => H.
       inversion H => {H}; subst. 
@@ -349,46 +308,42 @@ Proof.
         apply/LResP => //.
         move:H4 => /=.
         apply/contra_not => Hyp.
-        apply/(free_in_subst_inv) => //=.
+        apply/(free_in_subst) => //=.
       + apply/LParPR => //=.
-        apply/(lin_subst_inv _ (subst_ch
-            (fun i => var_ch (shift (shift i))) (var_ch i))).
-        apply/H4. 
-        rewrite/injectiveNS => j _.
+        apply/(lin_subst_inv _ (shift (shift x)) _
+                 (fun w =>  (shift (shift w)))) => //.
+        move => z _.
         by case.
-        by asimpl.
     }
-  - move => n0 R i. (* swapC *) 
+  - move => n0 R x. (* swapC *) 
     split. 
     {
       move => H. 
       inversion H;subst. 
       constructor => /=.
-      apply/(lin_subst (shift (shift i)) _ _ (swap_ch var_zero var_one)) => //.
+      apply/(lin_subst (shift(shift x)) _ _ (swap_ch zero one)) => //.
       apply/injectiveNS_swap.
     }
     {
       move => H.
       inversion H; subst. 
       constructor. 
-      apply/lin_subst_inv.
+      apply/(lin_subst_inv (shift(shift x)) _ _
+               (swap_ch zero one)) => //.
       apply/H2. 
       apply/injectiveNS_swap.
-      by asimpl.
     } 
-  - move => R. (* swapB *)
+  - move => n0. (* swapB *)
     split.
     {
       move => H.
       inversion H;subst. 
       inversion H2;subst. 
       constructor; constructor => /=.
-      apply/(lin_subst ) => //.
-      apply/(lin_subst ) => //.
-      apply/H3. 
+      apply/(lin_subst (shift (shift (shift (shift x))))) => //.
+      apply/(lin_subst (shift (shift (shift (shift x))))) => //.
       apply/injectiveNS_swap.
       apply/injectiveNS_swap.
-      by asimpl.
     }
     {
       move => H. 
@@ -396,13 +351,17 @@ Proof.
       inversion H2; subst. 
       constructor. 
       constructor => /=. 
-      apply/(lin_subst_inv). 
-      apply/(lin_subst_inv (shift (shift (shift (shift i))))). 
-      apply/H3. 
+      apply (lin_subst_inv (shift( shift (shift (shift x))))
+               ((swap_ch zero two) (shift( shift (shift (shift x)))))
+               _ (swap_ch zero two)) => //.
+      apply (lin_subst_inv 
+               ((swap_ch zero two) (shift( shift (shift (shift x)))))
+               ((swap_ch one three)
+                  ((swap_ch zero two)
+                     (shift( shift (shift (shift x))))))
+               _ (swap_ch one three)) => //.
       apply/injectiveNS_swap.
-      by asimpl.
       apply/injectiveNS_swap.
-      by asimpl.
     }
   - split.
     move => H.
@@ -410,42 +369,42 @@ Proof.
     inversion H2.
     move => H.
     inversion H.     
-  - move => n0 P0 Q0 H1 H2 i. 
+  - move => n0 P0 Q0 H1 H2 x. 
     by apply iff_sym.
-  - move => n0 P0 Q0 R Heq H1 Heq2 H2 i.
-    by rewrite H1. 
+  - move => n0 P0 Q0 R Heq H1 Heq2 H2 x.
+    firstorder. 
   - move => n0 P0 P' Q0 Q' Heq1 H1 Heq2 H2 i.
     split. 
     * move => Hyp.
       inversion Hyp; subst. 
-      apply/LParPL. 
-      by rewrite -H1. 
+      apply/LParPL.
+      firstorder. 
       move: H5; apply/contra_not => Hyp'. 
       by apply/(free_in_congruence _ _ Q'). 
       apply/LParPR. 
       move: H4; apply/contra_not => Hyp'. 
       by apply/(free_in_congruence _ _ P'). 
-      by rewrite -H2.
+      firstorder.
     * move => Hyp.
       inversion Hyp; subst. 
       apply/LParPL. 
-      by rewrite H1. 
+      firstorder.
       move: H5; apply/contra_not => Hyp'. 
       apply/(free_in_congruence _ Q0) => //. 
       apply/LParPR. 
       move: H4; apply/contra_not => Hyp'. 
       apply/(free_in_congruence _ P0) => //. 
-      by rewrite H2.
+      firstorder. 
   - move => n0 P0 P' Heq H i.
     split. 
     * move => Hyp.
       inversion Hyp; subst. 
       apply/LResP. 
-      by rewrite -H. 
+      firstorder.
     * move => Hyp.
       inversion Hyp; subst. 
       apply/LResP. 
-      by rewrite H. 
+      firstorder. 
   - move => n0 P0 P' x Heq H i.
     split. 
     * move => Hyp.
@@ -454,14 +413,14 @@ Proof.
       move: H2; apply/contra_not => Hyp'. 
       apply/(free_in_congruence _ _ P') => //.
       apply/LClosePcongr => //.
-      by rewrite -H.
+      firstorder. 
     * move => Hyp.
       inversion Hyp; subst. 
       apply/LCloseP. 
       move: H2; apply/contra_not => Hyp'. 
       apply/(free_in_congruence _ P0) => //.
       apply/LClosePcongr => //.
-      by rewrite H.
+      firstorder. 
   - move => n0 P0 P' x Heq H i.
     split. 
     * move => Hyp.
@@ -470,27 +429,27 @@ Proof.
       move: H2; apply/contra_not => Hyp'. 
       apply/(free_in_congruence _ _ P') => //.
       apply/LWaitPcongr => //.
-      by rewrite -H.
+      firstorder. 
     * move => Hyp.
       inversion Hyp; subst. 
       apply/LWaitP. 
       move: H2; apply/contra_not => Hyp'. 
       apply/(free_in_congruence _ P0) => //.
       apply/LWaitPcongr => //.
-      by rewrite H.
+      firstorder. 
   - move => n0 P0 P' x y Heq H i.
     split. 
     * move => Hyp.
       inversion Hyp; subst. 
       apply/LDelP => //. 
-      by rewrite -H.
+      firstorder. 
       apply/LDelPObj => //.
       move:H5; apply/contra_not => Hyp'.
       by apply/(free_in_congruence _ _ P'). 
     * move => Hyp.
       inversion Hyp; subst. 
       apply/LDelP => //. 
-      by rewrite H.
+      firstorder. 
       apply/LDelPObj => //.
       move:H5; apply/contra_not => Hyp'.
       by apply/(free_in_congruence _ P0). 
@@ -499,45 +458,12 @@ Proof.
     * move => Hyp.
       inversion Hyp; subst. 
       apply/LInSP => //. 
-      by rewrite -H.
+      firstorder. 
     * move => Hyp.
       inversion Hyp; subst. 
       apply/LInSP => //. 
-      by rewrite H.
+      firstorder. 
 Qed.
-
-
-(* Useful Lemma *) 
-
-
-Lemma lin_then_free {n : nat} : forall x (P : proc n),
-    lin x P -> free_in x P.
-Proof. 
-  move => x P; elim: P x => /=.
-  - move => n0 x H; inversion H.
-  - move => n0 [i] P IH [j] H.
-    inversion H; subst.
-    by left. 
-    by right; apply/IH.
-  - move => n0 [i] P IH [j] H.
-    inversion H; subst.
-    by left. 
-    by right; apply/IH.
-  - move => n0 P IH [j] /= H.
-    inversion H; subst. 
-    by apply/IH.
-  - move => n0 P IH1 Q IH2 [i] H.
-    inversion H; subst. 
-    by left; apply/IH1.
-    by right; apply/IH2. 
-  - move => n0 [i] P IH [j] /= H.
-    inversion H; subst. 
-    by right; apply/IH. 
-  - move => n0 c c0 P IH x H.
-    inversion H; subst. 
-    by right; right; apply/IH.
-    by right; left. 
-Qed. 
 
 Lemma lin_free_in_wait {n : nat} : forall x y (P Q : proc n.+2),
     lin x (y ! ․ P ∥ x ? ․ Q) -> ~(free_in x P \/ free_in x Q). 
@@ -568,3 +494,5 @@ Proof.
     apply/contra_not.
     by move => _ /=; left. 
 Qed. 
+
+
