theories/typing.v
@@ -1,55 +1,54 @@
 (* Imported libraries *) 
 From mathcomp Require Import all_ssreflect.
 From Coq Require Import FunctionalExtensionality.
-(* Require Import Stdlib.Program.Equality. *)
-Require Import free_names types semantics syntax fintype core linearity_predicate env.
+From Coq Require Import Classical_Prop.
 
+Require Import free_names types synsem linearity_predicate env.
 
 (* Some extra injectiveNS properties that we may remove if we go into injectiveS instead *) 
 
-Lemma injectiveNS_scons_shift_var_zero {n : nat} : forall x P,
-    not(x=var_ch var_zero) -> 
-    injectiveNS (@shift n.+2 var_zero) P (scons x ids).
+Lemma injectiveNS_scons_shift_zero {n : nat} : forall x P,
+    not(x=  zero) -> 
+    injectiveNS (@shift n.+2 zero) P (scons x id_ren).
 Proof.
   move => x P H1.
-  rewrite/injectiveNS/shift/scons => j H2 => /=. 
+  rewrite/injectiveNS/shift/scons/id_ren => j H2 => /=. 
   destruct j.
-  destruct f => //.
-  destruct x; destruct f => //.
+  destruct c => //.
+  destruct x. destruct c => //.
+  congruence.
 Qed. 
 
-
-Lemma injectiveNS_scons_shift_var_one {n : nat} : forall x P,
-    not(x=var_ch var_one) -> 
-    injectiveNS (@shift n.+2 var_one) P (scons x ids).
+Lemma injectiveNS_scons_shift_one {n : nat} : forall x P,
+    not(x=  one) -> 
+    injectiveNS (@shift n.+2 one) P (scons x id_ren).
 Proof.
   move => x P H1.
-  rewrite/injectiveNS/shift/scons => j H2 => /=. 
+  rewrite/injectiveNS/shift/scons/id_ren => j H2 => /=. 
   destruct j.
-  destruct f => //.
-  destruct x; destruct f => //.
-  simpl.
-  move => H; subst. 
-  by move:H1; case.  
+  destruct c => //.
+  destruct x; destruct c => //.
+  congruence.
 Qed. 
-  
-Notation "x '!->' v ';' m" := (update m x v)
-                              (at level 100, v at next level, right associativity).
+
 (* Typing rules *)
 Reserved Notation "Delta ⊢ P"  (at level 40).
 
 (* StartTY *)
 Inductive OFT {n : nat} (Delta : env n) : proc n -> Prop :=  
-    TEndP : Delta ⊢ ∅
+    TEndP : Delta ⊢ EndP n
+    
   | TParP : forall P1 P2 : proc n,
             Delta ⊢ P1 -> Delta ⊢ P2 -> Delta ⊢ (P1 ∥ P2)
+ 
   | TResP : forall (T : sType) (P : proc n.+2),
-            (free_in (n.+2__ch var_zero) P ->
-             lin (n.+2__ch var_zero) P) ->
-            (free_in (n.+2__ch var_one) P ->
-             lin (n.+2__ch var_one) P) ->
+            (free_in zero P ->
+             lin zero P) ->
+            (free_in one P ->
+             lin one P) ->
             (T ::: (dual T ::: Delta)) ⊢ P ->
             Delta ⊢ ((ν) P)
+            
   | TWaitP : forall (x : ch n) (P : proc n),
              Delta x = end? ->
              Delta ⊢ P -> Delta ⊢ (x ? ․ P)
@@ -58,16 +57,16 @@ Inductive OFT {n : nat} (Delta : env n) : proc n -> Prop :=
               Delta ⊢ P -> Delta ⊢ (x ! ․ P)
   | TInSP : forall (x : ch n) (T' T : sType) (P : proc n.+1),
             Delta x = ? T ․ T' ->
-            lin (n.+1__ch var_zero) P ->
-            (T ::: (x !-> T'; Delta)) ⊢ P ->
+            lin ( zero) P ->
+            (T ::: (x !!-> T'; Delta)) ⊢ P ->
             Delta ⊢ (x ? (_)․P)
   | TDelP : forall (x y : ch n) (T' T : sType) (P : proc n),
             Delta x = ! T ․ T' ->
             Delta y = T ->
-            (x !-> T'; Delta) ⊢ P ->
+            (x !!-> T'; Delta) ⊢ P ->
             Delta ⊢ (x ! y ․ P)
             where  "Delta ⊢ P" := (OFT Delta P).
-            
+(* EndTY *)
 
 Lemma substitution {n m : nat} : forall (Delta: env n) (Gamma: env m) sigma P,
     injectiveS P sigma -> 
@@ -75,67 +74,59 @@ Lemma substitution {n m : nat} : forall (Delta: env n) (Gamma: env m) sigma P,
 Proof. 
   move => Delta Gamma sigma P; elim: P m Delta Gamma sigma.
   - constructor. 
-  - move => n0 [i] P IH m Delta Gamma sigma Hinj Hltc H => /=.
+  - move => n0 c P IH m Delta Gamma sigma Hinj Hltc H => /=.
     inversion H; subst. 
     apply/TWaitP.
     rewrite -H2; symmetry; apply/Hltc => /=.
     by left.
     apply/(IH _ Delta) => //.
-    rewrite/injectiveS => i0 j Hyp1 Hyp2 Hyp3.
-    apply/Hinj => //=.
-    by right. 
-    by right. 
-    by apply/(ltc_WaitP _ (var_ch i)). 
-  - move => n0 [i] P IH m Delta Gamma sigma Hinj Hltc H => /=.
+    rewrite/injectiveS => i0 j Hyp1 Hyp2 Hyp3; try tauto.
+    apply/Hinj => //=; try tauto.  
+   by apply/(ltc_WaitP _ (  c)). 
+  - move => n0 c P IH m Delta Gamma sigma Hinj Hltc H => /=.
     inversion H; subst. 
     apply/TCloseP.
     rewrite -H2; symmetry; apply/Hltc => /=.
     by left.
     apply/(IH _ Delta) => //.
     rewrite/injectiveS => i0 j Hyp1 Hyp2 Hyp3.
-    apply/Hinj => //=.
-    by right. 
-    by right. 
-    by apply/(ltc_CloseP _ (var_ch i)). 
+    apply/Hinj => //=; try tauto.
+    by apply/(ltc_CloseP _ (  c)). 
   - move => n0 P IH m Delta Gamma sigma Hinj Hltc H => /=.
     inversion H; subst. 
     apply/(TResP _ T).
     * move => Hyp.
       apply/lin_subst.
       apply/H1. 
-      apply/free_in_subst.
+      apply/free_in_subst_inv.
       apply/Hyp.
-      apply/injectiveNS_up_ch_ch_zero2.
-      apply/injectiveNS_up_ch_ch_zero2.
-      by simpl.
+      apply/injectiveNS_up_ch_zero2.
+      apply/injectiveNS_up_ch_zero2.
+      auto.
     * move => Hyp.
       apply/lin_subst. 
       apply/H2. 
-      apply/free_in_subst. 
+      apply/free_in_subst_inv. 
       apply/Hyp.
-      apply/injectiveNS_up_ch_ch_one.
-      apply/injectiveNS_up_ch_ch_one.
-      by simpl.
+      apply/injectiveNS_up_ch_one.
+      apply/injectiveNS_up_ch_one.
+      auto.
     * apply (IH _ (shift_env T (shift_env (dual T) Delta))
                (shift_env T (shift_env (dual T) Gamma))) => //.
       apply/injectiveS_ResP => //.
       apply/ltc_ResP => //.
   - move => n0 P IH1 Q IH2 m2 Delta Gamma sigma Hinj Hltc H => /=.
-    inversion H; subst. 
+    inversion H; subst; clear H. 
     constructor.
     + apply/(IH1 _ Delta) => //.
       rewrite/injectiveS => i0 j Hyp1 Hyp2 Hyp3.
-      apply/Hinj => //=.
-      by left.
-      by left. 
+      apply/Hinj => //=; try tauto.
       by apply/(ltc_ParPL _ _ Q).
     + apply/(IH2 _ Delta) => //.
       rewrite/injectiveS => i0 j Hyp1 Hyp2 Hyp3.
-      apply/Hinj => //=.
-      by right.
-      by right.
+      apply/Hinj => //=; try tauto.
       by apply/(ltc_ParPR _ P).
-  - move => n0 [i] P IH m Delta Gamma sigma Hinj Hltc H => /=.
+  - move => n0 c P IH m Delta Gamma sigma Hinj Hltc H => /=.
     inversion H; subst. 
     apply/(TInSP _ _ T' T).
     rewrite -H2. 
@@ -143,16 +134,16 @@ Proof.
     by apply/Hltc => /=; left. 
     apply/lin_subst.
     apply/H3. 
-    apply/injectiveNS_up_ch_ch_zero1. 
+    apply/injectiveNS_up_ch_zero1. 
     by simpl.
-    apply/(IH _ (shift_env T (update Delta (var_ch i) T'))) => //.
-    apply/(injectiveS_InSP (var_ch i)) => //.
-    apply (ltc_InSP _ _ (var_ch i)). 
+    apply/(IH _ (shift_env T (c !!-> T'; Delta))) => //.
+    apply/(injectiveS_InSP c) => //.
+    apply (ltc_InSP _ _ c). 
     apply/ltc_update => //=. (* here use injectiveS *)
     by left. 
-  - move => n0 [i] [j] P IH m Delta Gamma sigma Hinj Hltc H => /=.
+  - move => n0 c c0 P IH m Delta Gamma sigma Hinj Hltc H => /=.
     inversion H; subst. 
-    apply (TDelP _ _ _ T' (Delta (var_ch j))).
+    apply (TDelP _ _ _ T' (Delta c0) ).
     rewrite -H3. 
     symmetry.
     apply Hltc => /=.
@@ -160,9 +151,9 @@ Proof.
     symmetry.
     apply/Hltc => //=.
     by right; left. 
-    apply/(IH _ (update Delta (var_ch i) T')) => //.
-    apply/(injectiveS_DelP (var_ch i) (var_ch j)) => //.
-    apply/(ltc_DelP _ (var_ch i) (var_ch j)).
+    apply/(IH _ (c !!-> T'; Delta)) => //.
+    apply/(injectiveS_DelP c c0) => //.
+    apply/(ltc_DelP _ c c0).
     apply/ltc_update => //=. (* here use injectiveS *)
     by left.
 Qed. 
@@ -173,89 +164,76 @@ Lemma substitution_inv {n m : nat} : forall (Delta: env n) (Gamma: env m) sigma 
 Proof. 
   move => Delta Gamma sigma P; elim: P m Delta Gamma sigma.
   - constructor. 
-  - move => n0 [i] P IH m Delta Gamma sigma Hinj Hltc H => /=.
+  - move => n0 c P IH m Delta Gamma sigma Hinj Hltc H => /=.
     inversion H; subst. 
     apply/TWaitP.
     rewrite -H2; apply/Hltc => /=.
     by left.
     apply/(IH _ _ Gamma sigma) => //. 
-    rewrite/injectiveS => i0 j Hyp1 Hyp2 Hyp3.
-    apply/Hinj => //=.
-    by right. 
-    by right. 
-    by apply/(ltc_WaitP _ (var_ch i)). 
-  - move => n0 [i] P IH m Delta Gamma sigma Hinj Hltc H => /=.
+    move => x y Hyp1 Hyp2 Hyp3.
+    apply/Hinj => //=; try tauto.
+    by apply/(ltc_WaitP _ c). 
+  - move => n0 c P IH m Delta Gamma sigma Hinj Hltc H => /=.
     inversion H; subst. 
     apply/TCloseP.
     rewrite -H2; apply/Hltc => /=.
     by left.
     apply/(IH _ _ Gamma sigma) => //. 
-    rewrite/injectiveS => i0 j Hyp1 Hyp2 Hyp3.
-    apply/Hinj => //=.
-    by right. 
-    by right. 
-    by apply/(ltc_WaitP _ (var_ch i)). 
+    move => x y Hyp1 Hyp2 Hyp3.
+    apply/Hinj => //=; try tauto.
+    by apply/(ltc_WaitP _ c). 
   - move => n0 P IH m Delta Gamma sigma Hinj Hltc H => /=.
     inversion H; subst. 
     apply/(TResP _ T).
-    * move/(free_in_subst_inv _ (up_ch_ch (up_ch_ch sigma))) => Hyp. 
+    * move/(free_in_subst _ (up_ch (up_ch sigma))) => Hyp. 
       apply/lin_subst_inv => //.
       apply/H1 => //. 
-      apply/injectiveNS_up_ch_ch_zero2.
-    * move/(free_in_subst_inv _ (up_ch_ch (up_ch_ch sigma))) => Hyp. 
+      apply/injectiveNS_up_ch_zero2.
+    * move/(free_in_subst _ (up_ch (up_ch sigma))) => Hyp. 
       apply/lin_subst_inv => //.
       apply/H2 => //. 
-      apply/injectiveNS_up_ch_ch_one.
-    * apply (IH _ (shift_env T (shift_env (dual T) Delta))
-               (shift_env T (shift_env (dual T) Gamma)) 
-            (up_ch_ch (up_ch_ch sigma))) => //.
+      apply/injectiveNS_up_ch_one.
+    * apply (IH _ (T ::: ( (dual T) ::: Delta)) (T ::: ((dual T) ::: Gamma)) 
+               (up_ch (up_ch sigma))) => //.
       apply/injectiveS_ResP => //.
       apply/ltc_ResP => //.
   - move => n0 P IH1 Q IH2 m2 Delta Gamma sigma Hinj Hltc H => /=.
     inversion H; subst. 
     constructor.
     + apply/(IH1 _ Delta Gamma sigma) => //.
-      rewrite/injectiveS => i0 j Hyp1 Hyp2 Hyp3.
-      apply/Hinj => //=.
-      by left.
-      by left. 
+      move => x y Hyp1 Hyp2 Hyp3.
+      apply/Hinj => //=; try tauto.
       by apply/(ltc_ParPL _ _ Q).
     + apply/(IH2 _ Delta Gamma sigma) => //.
-      rewrite/injectiveS => i0 j Hyp1 Hyp2 Hyp3.
-      apply/Hinj => //=.
-      by right.
-      by right.
+      move => x y Hyp1 Hyp2 Hyp3.
+      apply/Hinj => //=; try tauto.
       by apply/(ltc_ParPR _ P).
-  - move => n0 [i] P IH m Delta Gamma sigma Hinj Hltc H.
+  - move => n0 c P IH m Delta Gamma sigma Hinj Hltc H.
     inversion H; subst. 
     apply/(TInSP _ _ T' T).
     rewrite -H2. 
     by apply/Hltc => /=; left. 
-    apply/(lin_subst_inv _ (var_ch var_zero) _ (up_ch_ch sigma)) => //.
-    apply/injectiveNS_up_ch_ch_zero1. 
-    apply/(IH _ (shift_env T (update Delta (var_ch i) T')) 
-             (shift_env T (update Gamma (sigma i) T')) (up_ch_ch sigma)) => //.
-    apply/(injectiveS_InSP (var_ch i)) => //.
-    apply (ltc_InSP _ _ (var_ch i)). 
+    apply/(lin_subst_inv _ zero _ (up_ch sigma)) => //.
+    apply/injectiveNS_up_ch_zero1. 
+    apply/(IH _ (T ::: (c !!-> T'; Delta)) (T ::: ((sigma c) !!-> T'; Gamma))
+             (up_ch sigma)) => //.
+    apply/(injectiveS_InSP c) => //.
+    apply (ltc_InSP _ _ c). 
     apply/ltc_update => //=. (* here use injectiveS *)
     by left. 
-
-  - move => n0 [i] [j] P IH m Delta Gamma sigma Hinj Hltc H => /=.
+  - move => n0 c c0 P IH m Delta Gamma sigma Hinj Hltc H => /=.
     inversion H; subst. 
-    apply/(TDelP _ _ _ T' (Gamma (sigma j))).
+    apply/(TDelP _ _ _ T' (Gamma (sigma c0))).
     rewrite -H3. 
     apply Hltc => /=.
     by left. 
-    apply/Hltc => //=.
-    by right; left. 
-
-    apply/(IH _ _ (update Gamma (sigma i) T') sigma) => //.
-    apply/(injectiveS_DelP (var_ch i) (var_ch j)) => //.
-    apply/(ltc_DelP _ (var_ch i) (var_ch j)).
+    apply/Hltc => //=; try tauto.
+    apply/(IH _ _ ((sigma c) !!-> T'; Gamma) sigma) => //.
+    apply/(injectiveS_DelP c c0) => //.
+    apply/(ltc_DelP _ c c0).
     apply/ltc_update => //=. (* here use injectiveS *)
     by left.
 Qed. 
-
 
 Theorem subject_congruence : forall n P Q Delta,
     @struct_eq n P Q -> OFT Delta P <-> OFT Delta Q. 
@@ -297,11 +275,13 @@ Proof.
         move/H1 => Hlin0.
         apply/LParPL => //.
         apply/free_in_0_shift.
+        
         by move/free_in_0_shift.
       + case. 
         move/H4 => Hlin1.
         apply/LParPL => //.
-        apply/free_in_1_shift.
+           apply/free_in_bounded_shift .
+        intros y cc.  inversion cc.
         by move/free_in_1_shift.       
       + apply/TParP => //.
         (* now we prove Delta ⊢ Q0 implies 
@@ -317,18 +297,16 @@ Proof.
       apply/TParP.
       + apply (TResP _ T) => //.
         * move => Hyp.
-          have : free_in (n0.+2__ch var_zero) (P0 ∥ shift_two_up Q0)
-            by left. 
+          have : free_in zero (P0 ∥ subst_proc (shift \o shift) Q0) by left. 
           move/H0 => HLin0.
           inversion HLin0; subst => //.
         * move => Hyp.
-          have : free_in (n0.+2__ch var_one) (P0 ∥ shift_two_up Q0)
-            by left. 
+          have : free_in one (P0 ∥ subst_proc (shift \o shift) Q0) by left. 
           move/H1 => HLin1.
           inversion HLin1; subst => //.
-      + move:H5 => /(substitution_inv _ _) => //.
+      + move:H5 => /substitution_inv => //.
         apply => //.
-        rewrite/injectiveS => i0 j Hyp1 Hyp2.
+        move => x y Hyp1 Hyp2.
         by case => ->.
     }
 
@@ -340,24 +318,23 @@ Proof.
       * move => Hyp.
         apply/lin_subst. 
         apply/H2.
-        apply/(free_in_subst _ (swap_ch var_zero var_one)) => //. 
+        apply/(free_in_subst_inv _ (swap_ch zero one)) => //. 
         apply/injectiveNS_swap.
         apply/injectiveNS_swap.
         auto. 
       * move => Hyp.
         apply/lin_subst. 
         apply/H1.
-        apply/(free_in_subst _ (swap_ch var_zero var_one)) => //. 
+        apply/(free_in_subst_inv _ (swap_ch zero one)) => //. 
         apply/injectiveNS_swap.
         apply/injectiveNS_swap.
         auto. 
       * apply (substitution (shift_env T (shift_env (dual T) Delta))) => //. 
         apply/injectiveS_swap.
-        have fact : 
-          (shift_env (dual T) (shift_env (dual (dual T)) Delta)) =
-            (swap_env (shift_env T (shift_env (dual T) Delta)) 
-               (var_ch var_zero) (var_ch var_one)).
-        { rewrite dual_dual_is_identity.
+        have fact : (dual T) ::: ((dual (dual T)) ::: Delta) =
+                      swap_env (T ::: ((dual T) ::: Delta)) zero one.
+        {
+          rewrite dual_dual_is_identity.
           apply functional_extensionality => x.
           rewrite/swap_env/shift_env.
           case: ifP.
@@ -367,8 +344,8 @@ Proof.
           move/eqP => -> //.
           move/eqP => Hyp'.
           destruct x => //.
-          destruct f => //.
-          destruct f => //. } 
+          destruct c => //.
+        } 
         rewrite fact. 
         apply/ltc_swap => //.
     }
@@ -377,20 +354,20 @@ Proof.
       inversion H; subst. 
       apply/(TResP _ (dual T)). 
       - move => Hyp.
-        apply/(lin_subst_inv _ (var_ch var_one) _ (swap_ch var_zero var_one)) => //.
+        apply/(lin_subst_inv _ (  one) _ (swap_ch zero one)) => //.
         apply/H2. 
         move: Hyp.
-        by move/(free_in_subst_inv _ (swap_ch var_zero var_one)).
+        by move/(free_in_subst _ (swap_ch zero one)).
         apply/injectiveNS_swap.
       - move => Hyp.
-        apply/(lin_subst_inv _ (var_ch var_zero) _ 
-                 (swap_ch var_zero var_one)) => //.
+        apply/(lin_subst_inv _ (  zero) _ 
+                 (swap_ch zero one)) => //.
         apply/H1. 
         move: Hyp.
-        by move/(free_in_subst_inv _ (swap_ch var_zero var_one)).
+        by move/(free_in_subst _ (swap_ch zero one)).
         apply/injectiveNS_swap.
-      - apply/(substitution_inv _ (shift_env T (shift_env (dual T) Delta))
-                 (swap_ch var_zero var_one)) => //.
+      - apply/(substitution_inv _ (T ::: ((dual T) ::: Delta))
+                 (swap_ch zero one)) => //.
         + apply/injectiveS_swap.
         + apply/ltc_swap.
           apply/functional_extensionality => x.
@@ -403,8 +380,7 @@ Proof.
           by move/eqP => ->.
           move/eqP => Hyp'.
           destruct x => //.
-          destruct f => //.
-          destruct f => //.
+          destruct c => //.
     }
 
   - split. (* SC_Res_SwapB *) 
@@ -415,59 +391,59 @@ Proof.
       apply/(TResP _ T0).
       * move => /= Hyp.
         apply/LResP => /=.
-        have:  free_in (n0.+4__ch var_zero) P0. 
+        have:  free_in zero P0. 
         { 
-          apply/(free_in_subst _ (swap_ch var_zero var_two)). 
-          apply/(free_in_subst _ (swap_ch var_one var_three)). 
+          apply/(free_in_subst_inv _ (swap_ch zero two)). 
+          apply/(free_in_subst_inv _ (swap_ch one three)). 
           apply/Hyp.
           apply/injectiveNS_swap.
           apply/injectiveNS_swap.
         }
         move/H4 => H'.
-        apply/(lin_subst (shift (shift var_zero))) => //.
-        apply/(lin_subst var_zero) => //.
+        apply/(lin_subst (shift (shift zero))) => //.
+        apply/(lin_subst zero) => //.
         apply/injectiveNS_swap.
         apply/injectiveNS_swap.
       * move => /= Hyp.
         apply/LResP => /=.
-        have:  free_in (n0.+4__ch var_one) P0. 
-        { apply/(free_in_subst _ (swap_ch var_zero var_two)). 
-          apply/(free_in_subst _ (swap_ch var_one var_three)) => //. 
+        have:  free_in one P0. 
+        { apply/(free_in_subst_inv _ (swap_ch zero two)). 
+          apply/(free_in_subst_inv _ (swap_ch one three)) => //. 
           apply/injectiveNS_swap.
           apply/injectiveNS_swap. }
         move/H5 => H'.
-        apply/(lin_subst var_one) => //.
-        apply/(lin_subst var_one) => //.
+        apply/(lin_subst one) => //.
+        apply/(lin_subst one) => //.
         apply/injectiveNS_swap.
         apply/injectiveNS_swap.
       * apply/(TResP _ T).
         + move => /= Hyp. 
-          have : free_in (n0.+4__ch (shift (shift var_zero))) P0. 
-          { apply/(free_in_subst _ (swap_ch var_zero var_two)). 
-            apply/(free_in_subst _ (swap_ch var_one var_three)) => //.
+          have : free_in ((shift (shift zero))) P0. 
+          { apply/(free_in_subst_inv _ (swap_ch zero two)). 
+            apply/(free_in_subst_inv _ (swap_ch one three)) => //.
             apply/injectiveNS_swap.
             apply/injectiveNS_swap. }
           move/H1 => H'.
           inversion H'; subst. 
-          apply/(lin_subst var_zero) => //.
+          apply/(lin_subst zero) => //.
           apply/lin_subst. 
           apply/H8.
           apply/injectiveNS_swap.
-          by rewrite/var_zero.
+          by rewrite/zero.
           apply/injectiveNS_swap.
         + move => /= Hyp. 
-          have : free_in (n0.+4__ch (shift (shift var_one))) P0. 
-          { apply/(free_in_subst _ (swap_ch var_zero var_two)). 
-            apply/(free_in_subst _ (swap_ch var_one var_three)) => //.
+          have : free_in (shift (shift one)) P0. 
+          { apply/(free_in_subst_inv _ (swap_ch zero two)). 
+            apply/(free_in_subst_inv _ (swap_ch one three)) => //.
             apply/injectiveNS_swap.
             apply/injectiveNS_swap. }
           move/H2 => H'.
           inversion H'; subst. 
-          apply/(lin_subst var_three) => //.
+          apply/(lin_subst three) => //.
           apply/lin_subst. 
           apply/H8.
           apply/injectiveNS_swap.
-          by rewrite/var_one.
+          by rewrite/one.
           apply/injectiveNS_swap.
         + apply (substitution 
                    (shift_env T
@@ -483,15 +459,11 @@ Proof.
             case: ifP.
             move/eqP; case => -> //.
             move/eqP => Hyp.
-            destruct f => //.
-            destruct f => //.
-            destruct f => //.
-            destruct f => //.
+            destruct c => //.
+            destruct c => //.
+            destruct c => //.
           - apply/(substitution 
-                     (shift_env T0
-                      (shift_env (dual T0) 
-                         (shift_env T
-                            (shift_env (dual T) Delta))))) => //.
+                     (T0 ::: ((dual T0) ::: (T ::: ((dual T) ::: Delta))))) => //.
             apply/injectiveS_swap.
             apply/ltc_swap.
             apply/functional_extensionality => [x].
@@ -500,9 +472,8 @@ Proof.
             case: ifP. 
             move/eqP; case => -> //.
             move/eqP => Hyp.
-            destruct f => //.
-            destruct f => //.
-            destruct f => //.
+            destruct c => //.
+            destruct c => //.
     }
     { 
       move => H.
@@ -510,48 +481,48 @@ Proof.
       inversion H3; subst => {H3}.
       apply/(TResP _ T0).
       
-      + move/(free_in_subst_inv _ (swap_ch var_zero var_two)).
-        move/(free_in_subst_inv _ (swap_ch var_one var_three)).
+      + move/(free_in_subst _ (swap_ch zero two)).
+        move/(free_in_subst _ (swap_ch one three)).
         move/H0 => Hyp.
         apply/LResP.
-        apply/(lin_subst_inv _ _ _ (swap_ch var_zero var_two)) => //. 
-        apply/(lin_subst_inv _ _ _ (swap_ch var_one var_three)) => //.
+        apply/(lin_subst_inv _ _ _ (swap_ch zero two)) => //. 
+        apply/(lin_subst_inv _ _ _ (swap_ch one three)) => //.
         apply/Hyp.
         apply/injectiveNS_swap.
         apply/injectiveNS_swap.
 
-      + move/(free_in_subst_inv _ (swap_ch var_zero var_two)).
-        move/(free_in_subst_inv _ (swap_ch var_one var_three)).
+      + move/(free_in_subst _ (swap_ch zero two)).
+        move/(free_in_subst _ (swap_ch one three)).
         move/H4 => Hyp.
         apply/LResP.
-        apply/(lin_subst_inv _ _ _ (swap_ch var_zero var_two)) => //. 
-        apply/(lin_subst_inv _ _ _ (swap_ch var_one var_three)) => //.
+        apply/(lin_subst_inv _ _ _ (swap_ch zero two)) => //. 
+        apply/(lin_subst_inv _ _ _ (swap_ch one three)) => //.
         apply/Hyp.
         apply/injectiveNS_swap.
         apply/injectiveNS_swap.
 
       + apply/(TResP _ T).
-        * move/(free_in_subst_inv _ (swap_ch var_zero var_two)).
-          move/(free_in_subst_inv _ (swap_ch var_one var_three)).
+        * move/(free_in_subst _ (swap_ch zero two)).
+          move/(free_in_subst _ (swap_ch one three)).
           move/H1 => Hyp.
           inversion Hyp; subst. 
-          apply/(lin_subst_inv _ _ _ (swap_ch var_zero var_two)) => //.
-          apply/(lin_subst_inv _ (var_ch var_two) _ (swap_ch var_one var_three)) => //.
+          apply/(lin_subst_inv _ _ _ (swap_ch zero two)) => //.
+          apply/(lin_subst_inv _ (  two) _ (swap_ch one three)) => //.
           apply/injectiveNS_swap.
           apply/injectiveNS_swap.
-        * move/(free_in_subst_inv _ (swap_ch var_zero var_two)).
-          move/(free_in_subst_inv _ (swap_ch var_one var_three)).
+        * move/(free_in_subst _ (swap_ch zero two)).
+          move/(free_in_subst _ (swap_ch one three)).
           move/H2 => Hyp.
           inversion Hyp; subst. 
-          apply/(lin_subst_inv _ _ _ (swap_ch var_zero var_two)) => //.
-          apply/(lin_subst_inv _ (var_ch var_three) _ (swap_ch var_one var_three)) => //.
+          apply/(lin_subst_inv _ _ _ (swap_ch zero two)) => //.
+          apply/(lin_subst_inv _ (  three) _ (swap_ch one three)) => //.
           apply/injectiveNS_swap.
           apply/injectiveNS_swap.
 
         * apply/(substitution_inv _ 
                    (shift_env T0 (shift_env (dual T) 
                                    (shift_env T (shift_env (dual T0) Delta))))
-                   (swap_ch var_zero var_two)). 
+                   (swap_ch zero two)). 
           apply/injectiveS_swap.
           apply/ltc_swap.
           apply/functional_extensionality => [x].
@@ -560,13 +531,11 @@ Proof.
           case: ifP.
           move/eqP; case => -> //.
           move/eqP => Hyp.
-          destruct f => //.
-          destruct f => //.
-          destruct f => //.
+          destruct c => //.
+          destruct c => //.
           apply/(substitution_inv _ 
-                   (shift_env T0 (shift_env (dual T0) 
-                                   (shift_env T (shift_env (dual T) Delta))))
-                   (swap_ch var_one var_three)) => //. 
+                   (T0 ::: ((dual T0) ::: (T ::: ((dual T) ::: Delta))))
+                   (swap_ch one three)) => //. 
           apply/injectiveS_swap.
           apply/ltc_swap.
           apply/functional_extensionality => [x].
@@ -575,10 +544,9 @@ Proof.
           case: ifP.
           move/eqP; case => -> //.
           move/eqP => Hyp.
-          destruct f => //.
-          destruct f => //.
-          destruct f => //.
-          destruct f => //.
+          destruct c => //.
+          destruct c => //.
+          destruct c => //.
     }
 
   (* SC_Res_Zero *)
@@ -594,7 +562,6 @@ Proof.
   (* SC_Refl *) 
   - move => n0 P0 Q0 Hstruct IH Delta.
     by apply iff_sym.
-    
     
   (* SC_Sym *) 
   - move => n0 P0 Q0 R Heq1 H1 Heq2 H2 Delta.
@@ -689,8 +656,6 @@ Proof.
       by apply/H0.
 Qed. 
 
-
-
 Lemma lin_reduction {n : nat} : forall (x : ch n) (P Q : proc n) Delta,
     reduce P Q -> OFT Delta P -> lin x P -> lin x Q.
 Proof.
@@ -717,7 +682,7 @@ Proof.
     apply/(subject_congruence _ P0) => //. 
     apply/(lin_congruence P0) => //. 
   (* *) 
-  - move => n0 P0 Q0 [i] Delta HDelta H.
+  - move => n0 P0 Q0 c Delta HDelta H.
     inversion H; subst => {H}.
     apply/LResP.
     inversion H2; subst => {H2}. 
@@ -726,16 +691,14 @@ Proof.
       inversion H3; subst => {H3}.
       apply/H2. 
       move:H4 => /=.
-      apply/contra_not. 
-      by right. 
+      tauto.
     + (* LParR *)
       apply/LParPR => /=.
       move: H3 => /=.
-      apply/contra_not. 
-      by right. 
+      tauto.
       inversion H4; subst => {H4}. 
       apply/H2.
-  - move => n0 [i_sent] P0 Q0 [j_lin] Delta HDelta H. 
+  - move => n0 x_sent P0 Q0 y_lin Delta HDelta H. 
     inversion H; subst => {H}.
     apply/LResP => /=. 
     inversion H2; subst => {H2}.
@@ -743,57 +706,53 @@ Proof.
       inversion H3; subst => {H3} /=. 
       * (* LDelP *) 
         apply/LParPL => //. 
-        move:H4 => /=.
+        move:H4 => /=. 
         apply/contra_not => Hyp; right.
-        apply (free_in_subst _ (scons (var_ch i_sent) ids)) => //=.
+        apply (free_in_subst_inv _ (scons x_sent id_ren)) => //=.
         apply/injectiveNS_scons_shift.
-        move: H2. 
-        simpl.
-        by apply/contra_not => ->.
+        move: H2 => /=.
+        tauto.
       * (* LDelPObj *)
         apply/LParPR => //. 
-        have fact:  lin (n0.+3__ch var_zero) Q0.
+        have fact:  lin zero Q0.
         { inversion HDelta; subst. (* derive lin 0 Q0 *)
           inversion H3; subst.     (* derive lin 0 Q0 *)
           by inversion H8; subst. (* derive lin 0 Q0 *) 
         }
         apply/lin_key_subst => //.
-        move:H4. 
+        move:H4.
         apply/contra_not => /= H.
         by right. 
     + (* LParPR *) 
       inversion H4; subst => {H4}. 
       apply/LParPR. 
       move:H3 => /=.
-      apply/contra_not. 
-      by right; right. 
+      tauto.
       apply/lin_subst. 
       apply/H1. 
       apply/injectiveNS_scons_shift.
       move:H3 => /=.
       apply/contra_not => ->.
-      by right; left. 
+      tauto.
       by simpl.
 Qed.
 
-
 Lemma weakening {n : nat}: forall x T Delta (P : proc n),
-    not (free_in x P) -> OFT Delta P ->	OFT (update Delta x T) P. 
+    not (free_in x P) -> OFT Delta P ->	OFT (x !!-> T; Delta) P. 
 Proof. 
   move => x T Delta P; elim: P x T Delta => /=.
-  - move => n0 x T Delta _ _. 
-    apply/TEndP.
+  - constructor.
   - move => n0 c P IH x T Delta => /Decidable.not_or; case => Hyp1 Hyp2 Hyp3.
     inversion Hyp3; subst. 
     apply/TWaitP.
-    by rewrite -H1; apply/update_others.
+    by rewrite -H1; apply/t_update_others.
     apply/IH => //.
   - move => n0 c P IH x T Delta => /Decidable.not_or; case => Hyp1 Hyp2 Hyp3.
     inversion Hyp3; subst. 
     apply/TCloseP.
-    by rewrite -H1; apply update_others.
+    by rewrite -H1; apply/t_update_others.
     apply/IH => //.
-  - move => n0 P IH [i] T Delta H1 H2.
+  - move => n0 P IH c T Delta H1 H2.
     inversion H2; subst. 
     apply/(TResP _ T0) => //.
     repeat rewrite shift_env_update. 
@@ -804,30 +763,29 @@ Proof.
     apply/TParP.
     apply/IH1 => //.
     apply/IH2 => //.
-  - move => n0 [i] P IH [j] T Delta =>/Decidable.not_or; 
+  - move => n0 c P IH y T Delta =>/Decidable.not_or; 
             case => H1 H2 H3.
     inversion H3; subst. 
     apply/(TInSP _ _ T' T0) => //.
-    rewrite/update. 
+    rewrite/t_update. 
     case: ifP => /eqP => //. 
-    case => H; subst => //. 
-    rewrite update_swap. 
+    rewrite t_update_swap. 
     rewrite shift_env_update.
     apply/IH => //.
     by symmetry.
-  - move => n0 [i] [i0] P IH [j] T Delta =>/Decidable.not_or.
+  - move => n0 c c0 P IH y T Delta =>/Decidable.not_or.
     case => H1 => /Decidable.not_or; case => H2 H3 H4. 
     inversion H4; subst. 
-    apply/(TDelP _ _ _ T' (Delta (var_ch i0))) => //.
-    rewrite/update. 
+    apply/(TDelP _ _ _ T' (Delta c0)) => //.
+    rewrite/t_update. 
     case: ifP => /eqP.
-    case => Hyp; subst => //.
+    move => Hyp; subst => //.
     move => _ //.
-    rewrite/update. 
+    rewrite/t_update. 
     case: ifP => /eqP.
-    case => Hyp; subst => //.
+    move => Hyp; subst => //.
     move => _ //.
-    rewrite update_swap.
+    rewrite t_update_swap.
     apply/IH => //.
     by symmetry.
 Qed. 
@@ -852,10 +810,10 @@ Proof.
     by apply/(free_in_reduction _ _ Q0).
     apply/IH => //.
     (* extra for extra condition below *) 
-    move => [i].
-    destruct i => //.
-    destruct f => //.
-    move:(Hlin (var_ch f)) => /= Hyp.
+    move => c.
+    destruct c => //.
+    destruct c => //.
+    move:(Hlin c) => /= Hyp.
     move/Hyp => H'.
     inversion H'; subst. 
     apply/H5.
@@ -889,9 +847,9 @@ Proof.
   (* R_Close *) 
   - move => n0 P0 Q0 _ Delta H.
     inversion H; subst. 
-    have fact1: lin (var_ch var_zero) (var_ch var_one ! ․ P0 ∥ var_ch var_zero ? ․ Q0) 
+    have fact1: lin (  zero) (  one ! ․ P0 ∥   zero ? ․ Q0) 
       by apply/H1; right; left.
-    have fact2: lin (var_ch var_one) (var_ch var_one ! ․ P0 ∥ var_ch var_zero ? ․ Q0)
+    have fact2: lin (  one) (  one ! ․ P0 ∥   zero ? ․ Q0)
       by apply/H2; left; left. 
     apply/(TResP _ T). 
     + move:fact1 => /lin_free_in_wait => /=.
@@ -907,54 +865,52 @@ Proof.
   (* R_Del *)
   - move => n0 x P0 Q0 Hlin Delta H.
     (* 
-      H = Delta ⊢ (ν) (var_one!x․P0 ∥ var_zero?(_)․Q0)
+      H = Delta ⊢ (ν) (one!x․P0 ∥ zero?(_)․Q0)
      *) 
     inversion H; subst.
     (* Inverting H, considering that TResP is invertible, we get
-       HLin0 = var_zero is linear
-       HLin1 = var_one is linear
-       H3 = T :: (dual T) Delta ⊢ (var_one!x․P0 ∥ var_zero?(_)․Q0)
+       HLin0 = zero is linear
+       HLin1 = one is linear
+       H3 = T :: (dual T) Delta ⊢ (one!x․P0 ∥ zero?(_)․Q0)
      *) 
     
     (* We now fix the linearity statememts *)
-    have HLin0: lin (var_ch var_zero)
-                  (var_ch var_one !x․P0 ∥ var_ch var_zero?(_)․Q0)
+    have HLin0: lin zero (one !x․P0 ∥   zero?(_)․Q0)
       by apply/H1; simpl; right; left.
-    have HLin1: lin (var_ch var_one)
-                  (var_ch var_one !x․P0 ∥ var_ch var_zero?(_)․Q0)
+    have HLin1: lin one (one !x․P0 ∥   zero?(_)․Q0)
       by apply/H2; left; left. 
     move => {H1 H2}. 
 
     (* --------------------------------------------------------- *)
     (* Below, from linearity of zero and one, we get some facts: *)
     (* --------------------------------------------------------- *)
-    have H_zero_not_in_P0: not (free_in (n0.+2__ch var_zero) P0).
+    have H_zero_not_in_P0: not (free_in zero P0).
     { 
       inversion HLin0; subst. 
       by move: H5 => /Decidable.not_or; case; case. 
       by move: H4; apply/contra_not => /= H'; right; right.
     }
     (**) 
-    have H_x_not_one: n0.+2__ch var_one <> x.
+    have H_x_not_one: one <> x.
     {
       inversion HLin1; subst. 
       by inversion H4; subst. 
       by move: H4 => /Decidable.not_or; case; case.
     }
     (**)
-    have H_one_not_in_Q0_scons: not (free_in (n0.+2__ch var_one) 
-                                       (subst_proc (scons x ids) Q0)).
+    have H_one_not_in_Q0_scons: not (free_in one
+                                       (subst_proc (scons x id_ren) Q0)).
     { 
       inversion HLin1; subst.
       move: H5; apply/contra_not => /= H'; right.
-      apply/free_in_subst. 
+      apply/free_in_subst_inv. 
       apply/H'.
-      apply/injectiveNS_scons_shift_var_one.
+      apply/injectiveNS_scons_shift_one.
       by rewrite/not => Hyp; subst. 
       by move: H4 => /Decidable.not_or; case; case. 
     }
     (**)
-    have H_x_not_zero: x <> n0.+2__ch var_zero.
+    have H_x_not_zero: x <> zero.
     {
       inversion HLin0; subst. 
       by move: H5 => /Decidable.not_or; case; case. 
@@ -967,25 +923,25 @@ Proof.
     (* Back to the typing judgenmets, we now invert H3 *) 
     inversion H3; subst.
     (* Inverting H3, considering that TParP is invertible, we get
-       H2 = T :: (dual T) Delta ⊢ var_one!x․P0
-       H4 = T :: (dual T) Delta ⊢ var_zero?(_)․Q0
+       H2 = T :: (dual T) Delta ⊢ one!x․P0
+       H4 = T :: (dual T) Delta ⊢ zero?(_)․Q0
      *)
 
 
     (* We now invert H4, the input side *) 
     inversion H4; simpl in *; subst; simpl in *.
-    rewrite update_var_zero in H7.
-    (* Inverting H4, considering var_zero?()․Q0 is invertible, we get 
+    rewrite update_zero in H7.
+    (* Inverting H4, considering zero?()․Q0 is invertible, we get 
        (for  T = ? T0 ․ T' ) 
        H6 : lin zero Q0
        H7 :  T0 :: T' :: !T0. (dual T') :: Delta ⊢ Q0
        therefore, also updating 
-       H2 : ? T0 ․ T' ::  ! T0 ․ dual T' Delta ⊢ var_one!x․P0
+       H2 : ? T0 ․ T' ::  ! T0 ․ dual T' Delta ⊢ one!x․P0
      *) 
     
     (* We now invert H2, the output side *) 
     inversion H2; simpl in *; subst; simpl in *.
-    rewrite update_var_one in H10.
+    rewrite update_one in H10.
     move: H8; case => H_x_T0 Htemp2; subst. 
     (* Inverting H2, we finally get:
        H10 :        ? T0 ․ T'   ::       (dual T') :: Delta ⊢ P0
@@ -995,15 +951,15 @@ Proof.
 
     apply/(TResP _ T') => /=.
 
-    + (* Prove var_zero is linear *)
+    + (* Prove zero is linear *)
       move => _.
       inversion HLin0; subst => {HLin0 HLin1}. 
       * move:H9 => /Decidable.not_or; case; case => //.
       * inversion H9; subst. 
         apply/LParPR => //. 
-        apply/(lin_subst (shift var_zero)) => //.
-        apply/injectiveNS_scons_shift_var_zero => //.
-    + (* Prove var_one is linear *)
+        apply/(lin_subst (shift zero)) => //.
+        apply/injectiveNS_scons_shift_zero => //.
+    + (* Prove one is linear *)
       move => _.
       inversion HLin1; subst => {HLin0 HLin1}. 
       * inversion H8; subst => //. 
@@ -1014,32 +970,29 @@ Proof.
       apply/TParP.
       * have Hweak : 
           shift_env T' (shift_env (dual T') Delta) =
-            update (shift_env (? T0 ․ T') (shift_env (dual T') Delta)) 
-                   (var_ch var_zero) T'.
+            (zero !!-> T';
+             (shift_env (? T0 ․ T') (shift_env (dual T') Delta))).
         apply/functional_extensionality => x0.
         destruct x0 => //; destruct f => //.
         rewrite Hweak.
         apply/weakening => //.
-      * move:H7 => /(weakening (var_ch var_two) (dual T')) => Hyp.
+      * move:H7 => /(weakening (  two) (dual T')) => Hyp.
         apply/substitution; last first. 
         apply/Hyp.
         move: H_one_not_in_Q0_scons.
         apply/contra_not.
-        move/free_in_subst_inv. 
+        move/free_in_subst. 
         apply.
-        rewrite update_var_two. 
+        rewrite update_two. 
         apply/ltc_scons. 
         rewrite H_x_T0. 
         destruct x => //=.
-        destruct f => //.
-        destruct f => //.
+        destruct o => //.
         (* below, extra because of extra requirements *) 
         destruct x. 
         apply/injectiveS_scons_shift => //.
-        destruct f => //.
-        destruct f => //.
-        move: (Hlin (var_ch f)).
-        simpl.
+        destruct o => //.
+        move: (Hlin c) => /=.
         have fact1 : forall (X Y Z : Prop), (X \/ Y -> Z) -> X -> Z
             by move => X Y Z Hyp1 Hyp2; apply: Hyp1; left.
         have fact2 : forall (X Y Z : Prop), (X \/ Y -> Z) -> Y -> Z
@@ -1047,11 +1000,11 @@ Proof.
         move/fact1 => /fact2 => /fact1. 
         move => MyH.
         have fact : 
-          lin (var_ch f)   
+          lin c
             (ResP
             (ParP 
-               (DelP (var_ch var_one) (var_ch (shift (shift f))) P0)
-               (InSP (var_ch var_zero) Q0))).
+               (DelP (  one) (  (shift (shift c))) P0)
+               (InSP (  zero) Q0))).
         apply/MyH.
         by rewrite/shift.
         inversion fact; subst. 
@@ -1061,5 +1014,6 @@ Proof.
         by right.
         move:H8 => /=. 
         apply/contra_not => H11.
-        by right; left.
+        tauto.
+        move => x  y _ _ => //.
 Qed. 
