README.md
@@ -1,7 +1,16 @@
 # rocq-session-types-tutorial
-A tutorial on how to mechanize session types in Rocq with Linearity Predicates 
+This is the code for the paper:
 
-## Compatibility
+_Mechanizing the Meta-Theory of Session Types in Rocq: a Tutorial._
+
+by Marco Carbone and Alberto Momigliano
+
+There are **2** versions of the implementation and accordingly of the paper describing it:
+
+1. The `main` branch with the current, maintained and simpler code
+2. The branch `tutorial-with-autosubsts2`, where the syntax was generated via Autosubst2 
+
+## Instructions
 
 It can be run either with Rocq 9.0.0 or with Coq Classic 8.20.1
 
@@ -10,3 +19,5 @@ It can be run either with Rocq 9.0.0 or with Coq Classic 8.20.1
 - `coq_makefile -f _CoqProject *.v -o Makefile; mv Makefile* theories; make`
 
 
+Whatever the version, you need to install the following Coq library:
+- all_ssreflect
